src/MicroSail/Symbolic/Mutator.v
@@ -1047,6 +1047,15 @@ Module Mutators
     | _   => dmut_fail "dmut_leakcheck" "Heap leak" h
     end.
 
+  Record Config : Type :=
+    MkConfig
+      { config_debug_function : forall Δ τ, 𝑭 Δ τ -> bool;
+      }.
+
+  Definition default_config : Config :=
+    {| config_debug_function _ _ f := false;
+    |}.
+
   Module DynMutV1.
 
     Fixpoint dmut_produce {Γ Σ} (asn : Assertion Σ) : DynamicMutator Γ Γ Unit Σ :=
@@ -1596,227 +1605,239 @@ Module Mutators
          end
       end.
 
-    Definition dmut_call_evar_debug {Γ Δ τ Σr} (f : 𝑭 Δ τ) (contract : SepContract Δ τ) (ts : NamedEnv (Term Σr) Δ) : DynamicMutator Γ Γ (fun Σ => Term Σ τ) Σr :=
-      fun Σ1 ζ1 pc1 s1 =>
-        outcome_debug
-          {| debug_call_logic_context          := Σ1;
-             debug_call_function_parameters    := Δ;
-             debug_call_function_result_type   := τ;
-             debug_call_function_name          := f;
-             debug_call_function_arguments     := subst ζ1 ts;
-             debug_call_function_contract      := contract;
-             debug_call_pathcondition          := pc1;
-             debug_call_program_context        := Γ;
-             debug_call_localstore             := symbolicstate_localstore s1;
-             debug_call_heap                   := symbolicstate_heap s1;
-          |}
-          (dmut_call_evar contract ts ζ1 pc1 s1).
+    Section WithConfig.
 
-    (* TODO: The code should be rewritten so this variable can be removed. *)
-    Parameter dummy : 𝑺.
+      Variable cfg : Config.
 
-    Fixpoint dmut_exec_evar {Γ τ Σ} (s : Stm Γ τ) {struct s} :
-      DynamicMutator Γ Γ (fun Σ => Term Σ τ) Σ :=
-      match s with
-      | stm_lit _ l => dmut_pure (term_lit τ l)
-      | stm_exp e => dmut_eval_exp e
-      | stm_let x τ s1 s2 =>
-        t1 <- dmut_exec_evar s1 ;;
-        dmut_push_local t1 ;;
-        t2 <- dmut_exec_evar s2 ;;
-        dmut_pop_local ;;
-        dmut_pure t2
-      | stm_block δ s =>
-        dmut_pushs_local (lift δ) ;;
-        t <- dmut_exec_evar s ;;
-        dmut_pops_local _ ;;
-        dmut_pure t
-      | stm_assign x s =>
-        t <- dmut_exec_evar s ;;
-        dmut_modify_local (fun _ ζ δ => δ ⟪ x ↦ subst ζ t ⟫)%env ;;
-        dmut_pure t
-      | stm_call f es =>
-        ts <- dmut_eval_exps es ;;
-        match CEnv f with
-        | Some c => dmut_call_evar_debug f c ts
-        | None   => dmut_fail "dmut_exec_evar" "Function call without contract" (f,ts)
-        end
-      | stm_call_frame δ s =>
-        δr <- dmut_get_local ;;
-        dmut_put_local (lift δ) ;;
-        dmut_bind_left (dmut_exec_evar s) (dmut_put_local δr)
-      | stm_call_external f es =>
-        ts <- dmut_eval_exps es ;;
-        dmut_call_evar (CEnvEx f) ts
-      | stm_if e s1 s2 =>
-        t__sc <- dmut_eval_exp e ;;
-        match term_get_lit t__sc with
-        | Some b =>
-          if b
-          then dmut_exec_evar s1
-          else dmut_exec_evar s2
-        | None =>
-          (dmut_assume_term t__sc ;; dmut_exec_evar s1) ⊗
-          (dmut_assume_term (term_not t__sc) ;; dmut_exec_evar s2)
-        end
-      | stm_seq s1 s2 => dmut_exec_evar s1 ;; dmut_exec_evar s2
-      | stm_assertk e1 _ k =>
-        t <- dmut_eval_exp e1 ;;
-        dmut_assume_term t ;;
-        dmut_exec_evar k
-      | stm_fail _ _ =>
-        dmut_block
-      | stm_match_list e s1 xh xt s2 =>
-        t <- dmut_eval_exp e ;;
-        (dmut_assume_formula
-           (formula_eq t (term_lit (ty_list _) nil));;
-         dmut_exec_evar s1) ⊗
-        (dmut_fresh
-           (𝑿to𝑺 xh) _ (dmut_fresh (𝑿to𝑺 xt) _
-           (dmut_assume_formula
-              (formula_eq (sub_term (sub_comp sub_wk1 sub_wk1) t)
-                          (term_binop binop_cons (@term_var _ _ _ (inctx_succ inctx_zero)) (@term_var _ _ _ inctx_zero)));;
-            dmut_push_local (@term_var _ _ _ (inctx_succ inctx_zero));;
-            dmut_push_local (@term_var _ _ _ inctx_zero);;
-            t2 <- dmut_exec_evar s2 ;;
-            dmut_pop_local ;;
-            dmut_pop_local ;;
-            dmut_pure t2)))
-      | stm_match_sum e xinl s1 xinr s2 =>
-        t__sc <- dmut_eval_exp e ;;
-        match term_get_sum t__sc with
-        | Some (inl t) =>
-          dmut_push_local t;;
-          dmut_bind_left (dmut_exec_evar s1) dmut_pop_local
-        | Some (inr t) =>
-          dmut_push_local t;;
-          dmut_bind_left (dmut_exec_evar s2) dmut_pop_local
-        | None =>
-          dmut_fresh _ _
-            (dmut_assume_formula
-               (formula_eq (sub_term sub_wk1 t__sc) (term_inl (@term_var _ (𝑿to𝑺 xinl) _ inctx_zero)));;
-             dmut_push_local (@term_var _ (𝑿to𝑺 xinl) _ inctx_zero);;
-             dmut_bind_left (dmut_exec_evar s1) dmut_pop_local) ⊗
-          dmut_fresh _ _
-            (dmut_assume_formula
-               (formula_eq (sub_term sub_wk1 t__sc) (term_inr (@term_var _ (𝑿to𝑺 xinr) _ inctx_zero)));;
-             dmut_push_local (@term_var _ (𝑿to𝑺 xinr) _ inctx_zero);;
-             dmut_bind_left (dmut_exec_evar s2) dmut_pop_local)
-        end
-      | stm_match_pair e xl xr s =>
-        t__sc <- dmut_eval_exp e ;;
-        match term_get_pair t__sc with
-        | Some (t1,t2) =>
-          dmut_push_local t1;;
-          dmut_push_local t2;;
+      Definition dmut_call_evar_debug {Γ Δ τ Σr} (f : 𝑭 Δ τ) (contract : SepContract Δ τ) (ts : NamedEnv (Term Σr) Δ) : DynamicMutator Γ Γ (fun Σ => Term Σ τ) Σr :=
+        fun Σ1 ζ1 pc1 s1 =>
+          let o := dmut_call_evar contract ts ζ1 pc1 s1 in
+          if config_debug_function cfg f
+          then outcome_debug
+                 {| debug_call_logic_context          := Σ1;
+                    debug_call_function_parameters    := Δ;
+                    debug_call_function_result_type   := τ;
+                    debug_call_function_name          := f;
+                    debug_call_function_arguments     := subst ζ1 ts;
+                    debug_call_function_contract      := contract;
+                    debug_call_pathcondition          := pc1;
+                    debug_call_program_context        := Γ;
+                    debug_call_localstore             := symbolicstate_localstore s1;
+                    debug_call_heap                   := symbolicstate_heap s1;
+                 |}
+                 o
+          else o.
+
+      Fixpoint dmut_exec_evar {Γ τ Σ} (s : Stm Γ τ) {struct s} :
+        DynamicMutator Γ Γ (fun Σ => Term Σ τ) Σ :=
+        match s with
+        | stm_lit _ l => dmut_pure (term_lit τ l)
+        | stm_exp e => dmut_eval_exp e
+        | stm_let x τ s1 s2 =>
+          t1 <- dmut_exec_evar s1 ;;
+          dmut_push_local t1 ;;
+          t2 <- dmut_exec_evar s2 ;;
+          dmut_pop_local ;;
+          dmut_pure t2
+        | stm_block δ s =>
+          dmut_pushs_local (lift δ) ;;
           t <- dmut_exec_evar s ;;
-          dmut_pop_local ;;
-          dmut_pop_local ;;
+          dmut_pops_local _ ;;
           dmut_pure t
-        | None =>
-          dmut_fresh (𝑿to𝑺 xl) _ (dmut_fresh (𝑿to𝑺 xr) _
-            (dmut_assume_formula
-               (formula_eq
-                  (sub_term (sub_comp sub_wk1 sub_wk1) t__sc)
-                  (term_binop binop_pair (@term_var _ (𝑿to𝑺 xl) _ (inctx_succ inctx_zero)) (@term_var _ (𝑿to𝑺 xr) _ inctx_zero)));;
-             dmut_push_local (@term_var _ _ _ (inctx_succ inctx_zero));;
-             dmut_push_local (@term_var _ _ _ inctx_zero);;
-             t <- dmut_exec_evar s ;;
-             dmut_pop_local ;;
-             dmut_pop_local ;;
-             dmut_pure t))
-        end
-      | stm_match_enum E e alts =>
-        t__sc <- dmut_eval_exp e ;;
-        match term_get_lit t__sc with
-        | Some K => dmut_exec_evar (alts K)
-        | None =>
-          dmut_demonic_finite
-            (𝑬𝑲 E)
-            (fun K =>
-               dmut_assume_formula (formula_eq t__sc (term_enum E K));;
-               dmut_exec_evar (alts K))
-        end
-      | stm_match_tuple e p s =>
-        ts <- dmut_pair (dmut_eval_exp e) (dmut_freshen_tuplepat p) ;;
-        let '(t__sc,(t__p,t__Δ)) := ts in
-        dmut_assume_formula (formula_eq t__sc t__p) ;;
-        dmut_pushs_local t__Δ ;;
-        t <- dmut_exec_evar s ;;
-        dmut_pops_local _ ;;
-        dmut_pure t
-      | stm_match_union U e alt__pat alt__rhs =>
-        t__sc <- dmut_eval_exp e ;;
-        match term_get_union t__sc with
-        | Some (existT K t__field) =>
-          dmut_freshen_pattern (alt__pat K) >>= (fun Σ2 ζ2 '(t__pat, δ__Δ) =>
-            dmut_assume_formula (formula_eq t__pat (sub_term ζ2 t__field));;
-            dmut_pushs_local δ__Δ;;
-            t__rhs <- dmut_sub ζ2 (dmut_exec_evar (alt__rhs K));;
-            dmut_pops_local _;;
-            dmut_pure t__rhs)
-        | None =>
-          dmut_demonic_finite
-            (𝑼𝑲 U)
-            (fun K =>
-               dmut_freshen_pattern (alt__pat K) >>= (fun Σ2 ζ2 '(t__pat, δ__Δ) =>
-               dmut_assume_formula (formula_eq (sub_term ζ2 t__sc) (term_union U K t__pat));;
-               dmut_pushs_local δ__Δ;;
-               t__rhs <- dmut_sub ζ2 (dmut_exec_evar (alt__rhs K));;
-               dmut_pops_local _;;
-               dmut_pure t__rhs))
-        end
-      | stm_match_record R e p s =>
-        ts <- dmut_pair (dmut_eval_exp e) (dmut_freshen_recordpat 𝑿to𝑺 p) ;;
-        let '(t__sc,(t__p,t__Δ)) := ts in
-        dmut_assume_formula (formula_eq t__sc t__p) ;;
-        dmut_pushs_local t__Δ ;;
-        t <- dmut_exec_evar s ;;
-        dmut_pops_local _ ;;
-        dmut_pure t
-      | stm_read_register reg =>
-        dmut_consume_chunk_evar (chunk_ptsreg reg (@term_var [(dummy,_)] dummy _ inctx_zero)) [None]%arg >>= fun Σ1 _ E1 =>
-        match snd (env_unsnoc E1) with
-        | Some t => dmut_produce_chunk (chunk_ptsreg reg t) ;; dmut_pure t
-        (* Extracting the points to chunk should never fail here. Because there is exactly one binding
-           in the ghost environment and the chunk matching will always instantiate it. *)
-        | None => dmut_fail "dmut_exec_evar" "You have found a unicorn." tt
-        end
-      | stm_write_register reg e =>
-        tnew <- dmut_eval_exp e ;;
-        dmut_consume_chunk_evar (chunk_ptsreg reg (@term_var _ dummy _ inctx_zero)) [None]%arg ;;
-        dmut_produce_chunk (chunk_ptsreg reg tnew) ;;
-        dmut_pure tnew
-      | stm_bind _ _ =>
-        dmut_fail "dmut_exec_evar" "stm_bind not supported" tt
-      | stm_debugk k =>
-        dmut_exec_evar k
-      end.
+        | stm_assign x s =>
+          t <- dmut_exec_evar s ;;
+          dmut_modify_local (fun _ ζ δ => δ ⟪ x ↦ subst ζ t ⟫)%env ;;
+          dmut_pure t
+        | stm_call f es =>
+          ts <- dmut_eval_exps es ;;
+          match CEnv f with
+          | Some c => dmut_call_evar_debug f c ts
+          | None   => dmut_fail "dmut_exec_evar" "Function call without contract" (f,ts)
+          end
+        | stm_call_frame δ s =>
+          δr <- dmut_get_local ;;
+          dmut_put_local (lift δ) ;;
+          dmut_bind_left (dmut_exec_evar s) (dmut_put_local δr)
+        | stm_call_external f es =>
+          ts <- dmut_eval_exps es ;;
+          dmut_call_evar (CEnvEx f) ts
+        | stm_if e s1 s2 =>
+          t__sc <- dmut_eval_exp e ;;
+          match term_get_lit t__sc with
+          | Some b =>
+            if b
+            then dmut_exec_evar s1
+            else dmut_exec_evar s2
+          | None =>
+            (dmut_assume_term t__sc ;; dmut_exec_evar s1) ⊗
+            (dmut_assume_term (term_not t__sc) ;; dmut_exec_evar s2)
+          end
+        | stm_seq s1 s2 => dmut_exec_evar s1 ;; dmut_exec_evar s2
+        | stm_assertk e1 _ k =>
+          t <- dmut_eval_exp e1 ;;
+          dmut_assume_term t ;;
+          dmut_exec_evar k
+        | stm_fail _ _ =>
+          dmut_block
+        | stm_match_list e s1 xh xt s2 =>
+          t <- dmut_eval_exp e ;;
+          (dmut_assume_formula
+             (formula_eq t (term_lit (ty_list _) nil));;
+           dmut_exec_evar s1) ⊗
+          (dmut_fresh
+             (𝑿to𝑺 xh) _ (dmut_fresh (𝑿to𝑺 xt) _
+             (dmut_assume_formula
+                (formula_eq (sub_term (sub_comp sub_wk1 sub_wk1) t)
+                            (term_binop binop_cons (@term_var _ _ _ (inctx_succ inctx_zero)) (@term_var _ _ _ inctx_zero)));;
+              dmut_push_local (@term_var _ _ _ (inctx_succ inctx_zero));;
+              dmut_push_local (@term_var _ _ _ inctx_zero);;
+              t2 <- dmut_exec_evar s2 ;;
+              dmut_pop_local ;;
+              dmut_pop_local ;;
+              dmut_pure t2)))
+        | stm_match_sum e xinl s1 xinr s2 =>
+          t__sc <- dmut_eval_exp e ;;
+          match term_get_sum t__sc with
+          | Some (inl t) =>
+            dmut_push_local t;;
+            dmut_bind_left (dmut_exec_evar s1) dmut_pop_local
+          | Some (inr t) =>
+            dmut_push_local t;;
+            dmut_bind_left (dmut_exec_evar s2) dmut_pop_local
+          | None =>
+            dmut_fresh _ _
+              (dmut_assume_formula
+                 (formula_eq (sub_term sub_wk1 t__sc) (term_inl (@term_var _ (𝑿to𝑺 xinl) _ inctx_zero)));;
+               dmut_push_local (@term_var _ (𝑿to𝑺 xinl) _ inctx_zero);;
+               dmut_bind_left (dmut_exec_evar s1) dmut_pop_local) ⊗
+            dmut_fresh _ _
+              (dmut_assume_formula
+                 (formula_eq (sub_term sub_wk1 t__sc) (term_inr (@term_var _ (𝑿to𝑺 xinr) _ inctx_zero)));;
+               dmut_push_local (@term_var _ (𝑿to𝑺 xinr) _ inctx_zero);;
+               dmut_bind_left (dmut_exec_evar s2) dmut_pop_local)
+          end
+        | stm_match_pair e xl xr s =>
+          t__sc <- dmut_eval_exp e ;;
+          match term_get_pair t__sc with
+          | Some (t1,t2) =>
+            dmut_push_local t1;;
+            dmut_push_local t2;;
+            t <- dmut_exec_evar s ;;
+            dmut_pop_local ;;
+            dmut_pop_local ;;
+            dmut_pure t
+          | None =>
+            dmut_fresh (𝑿to𝑺 xl) _ (dmut_fresh (𝑿to𝑺 xr) _
+              (dmut_assume_formula
+                 (formula_eq
+                    (sub_term (sub_comp sub_wk1 sub_wk1) t__sc)
+                    (term_binop binop_pair (@term_var _ (𝑿to𝑺 xl) _ (inctx_succ inctx_zero)) (@term_var _ (𝑿to𝑺 xr) _ inctx_zero)));;
+               dmut_push_local (@term_var _ _ _ (inctx_succ inctx_zero));;
+               dmut_push_local (@term_var _ _ _ inctx_zero);;
+               t <- dmut_exec_evar s ;;
+               dmut_pop_local ;;
+               dmut_pop_local ;;
+               dmut_pure t))
+          end
+        | stm_match_enum E e alts =>
+          t__sc <- dmut_eval_exp e ;;
+          match term_get_lit t__sc with
+          | Some K => dmut_exec_evar (alts K)
+          | None =>
+            dmut_demonic_finite
+              (𝑬𝑲 E)
+              (fun K =>
+                 dmut_assume_formula (formula_eq t__sc (term_enum E K));;
+                 dmut_exec_evar (alts K))
+          end
+        | stm_match_tuple e p s =>
+          ts <- dmut_pair (dmut_eval_exp e) (dmut_freshen_tuplepat p) ;;
+          let '(t__sc,(t__p,t__Δ)) := ts in
+          dmut_assume_formula (formula_eq t__sc t__p) ;;
+          dmut_pushs_local t__Δ ;;
+          t <- dmut_exec_evar s ;;
+          dmut_pops_local _ ;;
+          dmut_pure t
+        | stm_match_union U e alt__pat alt__rhs =>
+          t__sc <- dmut_eval_exp e ;;
+          match term_get_union t__sc with
+          | Some (existT K t__field) =>
+            dmut_freshen_pattern (alt__pat K) >>= (fun Σ2 ζ2 '(t__pat, δ__Δ) =>
+              dmut_assume_formula (formula_eq t__pat (sub_term ζ2 t__field));;
+              dmut_pushs_local δ__Δ;;
+              t__rhs <- dmut_sub ζ2 (dmut_exec_evar (alt__rhs K));;
+              dmut_pops_local _;;
+              dmut_pure t__rhs)
+          | None =>
+            dmut_demonic_finite
+              (𝑼𝑲 U)
+              (fun K =>
+                 dmut_freshen_pattern (alt__pat K) >>= (fun Σ2 ζ2 '(t__pat, δ__Δ) =>
+                 dmut_assume_formula (formula_eq (sub_term ζ2 t__sc) (term_union U K t__pat));;
+                 dmut_pushs_local δ__Δ;;
+                 t__rhs <- dmut_sub ζ2 (dmut_exec_evar (alt__rhs K));;
+                 dmut_pops_local _;;
+                 dmut_pure t__rhs))
+          end
+        | stm_match_record R e p s =>
+          ts <- dmut_pair (dmut_eval_exp e) (dmut_freshen_recordpat 𝑿to𝑺 p) ;;
+          let '(t__sc,(t__p,t__Δ)) := ts in
+          dmut_assume_formula (formula_eq t__sc t__p) ;;
+          dmut_pushs_local t__Δ ;;
+          t <- dmut_exec_evar s ;;
+          dmut_pops_local _ ;;
+          dmut_pure t
+        | stm_read_register reg =>
+          let x := fresh Σ None in
+          dmut_consume_chunk_evar (chunk_ptsreg reg (@term_var [(x,_)] x _ inctx_zero)) [None]%arg >>= fun Σ1 _ E1 =>
+          match snd (env_unsnoc E1) with
+          | Some t => dmut_produce_chunk (chunk_ptsreg reg t) ;; dmut_pure t
+          (* Extracting the points to chunk should never fail here. Because there is exactly one binding
+             in the ghost environment and the chunk matching will always instantiate it. *)
+          | None => dmut_fail "dmut_exec_evar" "You have found a unicorn." tt
+          end
+        | stm_write_register reg e =>
+          let x := fresh Σ None in
+          tnew <- dmut_eval_exp e ;;
+          dmut_consume_chunk_evar (chunk_ptsreg reg (@term_var _ x _ inctx_zero)) [None]%arg ;;
+          dmut_produce_chunk (chunk_ptsreg reg tnew) ;;
+          dmut_pure tnew
+        | stm_bind _ _ =>
+          dmut_fail "dmut_exec_evar" "stm_bind not supported" tt
+        | stm_debugk k =>
+          dmut_exec_evar k
+        end.
 
-    Definition dmut_contract {Δ τ} (c : SepContract Δ τ) (s : Stm Δ τ) : DynamicMutator Δ Δ Unit (sep_contract_logic_variables c) :=
-      match c with
-      | MkSepContract _ _ Σ δ req result ens =>
-          DynMutV1.dmut_produce req ;;
-          dmut_exec_evar s      >>= fun Σ1 ζ1 t =>
-          dmut_consume_evar ens (subst (sub_snoc ζ1 (result,τ) t) (create_evarenv_id _)) ;;
-          dmut_leakcheck
-      end.
+      Definition dmut_contract {Δ τ} (c : SepContract Δ τ) (s : Stm Δ τ) : DynamicMutator Δ Δ Unit (sep_contract_logic_variables c) :=
+        match c with
+        | MkSepContract _ _ Σ δ req result ens =>
+            DynMutV1.dmut_produce req ;;
+            dmut_exec_evar s      >>= fun Σ1 ζ1 t =>
+            dmut_consume_evar ens (subst (sub_snoc ζ1 (result,τ) t) (create_evarenv_id _)) ;;
+            dmut_leakcheck
+        end.
 
-    Definition dmut_contract_outcome {Δ : PCtx} {τ : Ty} (c : SepContract Δ τ) (s : Stm Δ τ) :
-      Outcome DynamicMutatorError (DynamicMutatorResult Δ Unit (sep_contract_logic_variables c)) :=
-      let δ    := sep_contract_localstore c in
-      dmut_contract c s (sub_id _) nil (symbolicstate_initial δ).
+      Definition dmut_contract_outcome {Δ : PCtx} {τ : Ty} (c : SepContract Δ τ) (s : Stm Δ τ) :
+        Outcome DynamicMutatorError (DynamicMutatorResult Δ Unit (sep_contract_logic_variables c)) :=
+        let δ    := sep_contract_localstore c in
+        dmut_contract c s (sub_id _) nil (symbolicstate_initial δ).
+
+      Definition ValidContractDynMutWithConfig (Δ : PCtx) (τ : Ty)
+        (c : SepContract Δ τ) (body : Stm Δ τ) : Prop :=
+        outcome_safe (dmut_contract_outcome c body).
+
+    End WithConfig.
 
     Definition ValidContractDynMut (Δ : PCtx) (τ : Ty)
       (c : SepContract Δ τ) (body : Stm Δ τ) : Prop :=
-      outcome_safe (dmut_contract_outcome c body).
+      outcome_safe (dmut_contract_outcome default_config c body).
 
     Definition ValidContractDynMutReflect (Δ : PCtx) (τ : Ty)
                (c : SepContract Δ τ) (body : Stm Δ τ) : Prop :=
       is_true
         (outcome_ok (A := unit)
            (outcome_bind
-              (dmut_contract_outcome c body)
+              (dmut_contract_outcome default_config c body)
               (fun _ => outcome_block))).
 
     Lemma dynmutevarreflect_sound {Δ τ} (c : SepContract Δ τ) (body : Stm Δ τ) :
@@ -2925,9 +2946,6 @@ Module Mutators
          end
       end.
 
-    (* TODO: The code should be rewritten so this variable can be removed. *)
-    Parameter dummy : 𝑺.
-
     Fixpoint dmut_exec_evar {Γ τ Σ} (s : Stm Γ τ) {struct s} :
       DynamicMutator Γ Γ (fun Σ => Term Σ τ) Σ :=
       match s with
@@ -3088,7 +3106,8 @@ Module Mutators
         dmut_pops_local _ ;;
         dmut_pure t
       | stm_read_register reg =>
-        dmut_consume_chunk_evar (chunk_ptsreg reg (@term_var [(dummy,_)] dummy _ inctx_zero)) [None]%arg >>= fun Σ1 _ E1 =>
+        let x := fresh Σ None in
+        dmut_consume_chunk_evar (chunk_ptsreg reg (@term_var [(x,_)] x _ inctx_zero)) [None]%arg >>= fun Σ1 _ E1 =>
         match snd (env_unsnoc E1) with
         | Some t => dmut_produce_chunk (chunk_ptsreg reg t) ;; dmut_pure t
         (* Extracting the points to chunk should never fail here. Because there is exactly one binding
@@ -3096,8 +3115,9 @@ Module Mutators
         | None => dmut_fail "dmut_exec_evar" "You have found a unicorn." tt
         end
       | stm_write_register reg e =>
+        let x := fresh Σ None in
         tnew <- dmut_eval_exp e ;;
-        dmut_consume_chunk_evar (chunk_ptsreg reg (@term_var _ dummy _ inctx_zero)) [None]%arg ;;
+        dmut_consume_chunk_evar (chunk_ptsreg reg (@term_var _ x _ inctx_zero)) [None]%arg ;;
         dmut_produce_chunk (chunk_ptsreg reg tnew) ;;
         dmut_pure tnew
       | stm_bind _ _ =>
